fuck it we func

theories/Main.v
@@ -1,81 +1,45 @@
 From Coq Require Import Nat.
 From Coq Require Import Arith. Import Nat.
+From Coq Require Import Lists.List.
 From Coq Require Import Program.Basics.
 From Coq Require Import Lia.
 From Coq Require Import Bool.
 From Coq Require Import Strings.String.
-From Coq Require Import Lists.List. Import ListNotations.
+From Coq Require Import Strings.Ascii.
 From Coq Require Import Extraction.
 From Coq Require Import ExtrHaskellBasic.
 From Coq Require Import ExtrHaskellNatNum.
 From Coq Require Import ExtrHaskellString.
 
+
 Module Syntax.
 
-  Inductive AExpr : Type :=
-    | A_Const : nat -> AExpr
-    | A_Id : string -> AExpr
-    | A_Add : AExpr -> AExpr -> AExpr.
+  Inductive FExpr : Type :=
+  | F_Var : string -> FExpr
+  | F_Lambda : string -> FExpr -> FExpr
+  | F_Apply : FExpr -> Expr -> FExpr
+  | F_Cond : BExpr -> FExpr -> FExpr -> FExpr
+  | F_Let : string -> FExpr -> FExpr -> FExpr
+  | F_Return : Expr -> FExpr
 
-  Inductive LExpr {A : Type} : Type :=
-    | L_Id : string -> LExpr
-    | L_Nil : LExpr
-    | L_Cons : A -> LExpr -> LExpr.
+  with Expr : Type :=
+    | E_Bool : BExpr -> Expr
+    | E_Arith : AExpr -> Expr
 
-  Inductive BExpr : Type :=
+  with BExpr : Type :=
     | B_True : BExpr
     | B_False : BExpr
-    | B_Eq : AExpr -> AExpr -> BExpr
-    | B_Lt : AExpr -> AExpr -> BExpr
     | B_Not : BExpr -> BExpr
-    | B_And : BExpr -> BExpr -> BExpr.
+    | B_And : BExpr -> BExpr -> BExpr
+    | B_Le : AExpr -> AExpr -> BExpr
 
-  Inductive CExpr : Type :=
-    | C_Skip : CExpr
-    | C_Assign : string -> AExpr -> CExpr
-    | C_Seq : CExpr -> CExpr -> CExpr
-    | C_If : BExpr -> CExpr -> CExpr -> CExpr
-    | C_While : BExpr -> CExpr -> CExpr.
-
-  Coercion A_Id : string >-> AExpr.
-  Coercion A_Const : nat >-> AExpr.
-
-  Declare Custom Entry CExpr.
-  Declare Scope com_scope.
-
-  Notation "<{ e }>" := e (at level 0, e custom CExpr at level 99) : com_scope.
-  Notation "( x )" := x (in custom CExpr, x at level 99) : com_scope.
-  Notation "x" := x (in custom CExpr at level 0, x constr at level 0) : com_scope.
-  Notation "f x .. y" := (.. (f x) .. y)
-                    (in custom CExpr at level 0, only parsing,
-                    f constr at level 0, x constr at level 9,
-                    y constr at level 9) : com_scope.
-  Notation "x + y" := (A_Add x y) (in custom CExpr at level 50, left associativity) : com_scope.
-  Notation "'true'" := true (at level 1) : com_scope.
-  Notation "'true'" := B_True (in custom CExpr at level 0) : com_scope.
-  Notation "'false'" := false (at level 1) : com_scope.
-  Notation "'false'" := B_False (in custom CExpr at level 0) : com_scope.
-  Notation "x < y" := (B_Lt x y) (in custom CExpr at level 70, no associativity) : com_scope.
-  Notation "x = y" := (B_Eq x y) (in custom CExpr at level 70, no associativity) : com_scope.
-  Notation "x && y" := (B_And x y) (in custom CExpr at level 80, left associativity) : com_scope.
-  Notation "'~' b" := (B_Not b) (in custom CExpr at level 75, right associativity) : com_scope.
-  Notation "'skip'" :=
-      C_Skip (in custom CExpr at level 0) : com_scope.
-  Notation "x := y" :=
-    (C_Assign x y)
-      (in custom CExpr at level 0, x constr at level 0, y at level 85, no associativity) : com_scope.
-  Notation "x ; y" :=
-    (C_Seq x y)
-      (in custom CExpr at level 90, right associativity) : com_scope.
-  Notation "'if' x 'then' y 'else' z 'end'" :=
-    (C_If x y z)
-       (in custom CExpr at level 89, x at level 99,
-        y at level 99, z at level 99) : com_scope.
-  Notation "'while' x 'do' y 'end'" :=
-     (C_While x y)
-        (in custom CExpr at level 89, x at level 99, y at level 99) : com_scope.
-
-  Open Scope com_scope.
+  with AExpr : Type :=
+    | A_Const : nat -> AExpr
+    | A_Var : string -> AExpr
+    | A_Add : AExpr -> AExpr -> AExpr
+    | A_Sub : AExpr -> AExpr -> AExpr
+    | A_Mult : AExpr -> AExpr -> AExpr
+    | A_Func : FExpr -> AExpr.
 
 End Syntax.
 
@@ -84,69 +48,291 @@ Module Semantics.
 
   Notation "f <$> m" := (option_map f m) (at level 50, left associativity).
 
-  Fixpoint ap {A B : Type} (f : @Maybe (A -> B)) (m : @Maybe A) : @Maybe B :=
+  Fixpoint ap {A B : Type} (f : option (A -> B)) (m : option A) : option B :=
     match f with
-    | Nothing => Nothing
-    | Just f' => f' <$> m
+    | Some f' => f' <$> m
+    | None => None
     end.
 
   Notation "f <*> m" := (ap f m) (at level 50, left associativity).
 
-  Definition State := string -> @Maybe (nat + list nat).
-  Definition empty_state : State := fun _ => Nothing.
-  Definition update_state (s : State) (x : string) (n : nat + list nat) : State :=
-    fun y => if String.eqb x y then Just n else s y.
+  Inductive Env : Type :=
+  | EmptyEnv : Env
+  | ExtendEnv : string -> Value -> Env -> Env
+    with Value : Type :=
+    | V_Nat : nat -> Value
+    | V_Bool : bool -> Value
+    | V_Closure : FExpr -> Env -> Value
+    | V_ReturnValue : Value -> Value.
 
-  Fixpoint Aeval (e : AExpr) (s : State) : @Maybe (nat + list nat) :=
-    match e with
-    | A_Const n => Just (inl n)
-    | A_Id n => s n
-    | A_Add e1 e2 => (compose inl plus) <$> (Aeval e1 s) <*> (Aeval e2 s)
+
+  Example gpt : FExpr :=
+    F_Let "factorial" (F_Lambda "n"
+                    (F_Cond ((B_Le (A_Var "n") (A_Const 1)))
+                      (F_Return (E_Arith (A_Const 1)))
+                      (F_Return (E_Arith (A_Mult (A_Var "n") (A_Func (F_Apply (F_Var "factorial") (E_Arith (A_Sub (A_Var "n") (A_Const 1))))))))))
+      (F_Return (E_Arith (A_Func (F_Apply (F_Var "factorial") (E_Arith (A_Const 5)))))).
+
+
+  Fixpoint option_apply {A B : Type} (f : A -> option B) (x : option A) : option B :=
+    match x with
+    | Some x' => f x'
+    | None => None
     end.
 
-  Fixpoint Leval (e : LExpr) (s : State) : @Maybe (list nat) :=
-    match e with
-    | L_Id n => s n
-    | L_Nil => Just nil
-    | L_Cons e1 e2 => cons <$> (Aeval e1 s) <*> (Leval e2 s)
+  Inductive Either {A B : Type} : Type :=
+    | Right : B -> Either
+    | Left : A -> Either.
+
+  Definition either_map {A B C : Type} (f : A -> C) (either : Either) :=
+    match either with
+    | Right a => f a
+    | Left b => b
     end.
 
-  Fixpoint Beval (e : BExpr) (s : State) : @Maybe bool :=
-    match e with
-    | B_True => Just true
-    | B_False => Just false
-    | B_Eq e1 e2 => Nat.eqb <$> (Aeval e1 s) <*> (Aeval e2 s)
-    | B_Lt e1 e2 => Nat.ltb <$> (Aeval e1 s) <*> (Aeval e2 s)
-    | B_Not e => negb <$> Beval e s
-    | B_And e1 e2 => andb <$> (Beval e1 s) <*> (Beval e2 s)
+  Open Scope string_scope.
+
+  Fixpoint lookupEnv (env : Env) (varName : string) {struct env} : option Value :=
+    match env with
+    | EmptyEnv => None
+    | ExtendEnv name value restEnv =>
+        if String.eqb varName name
+        then Some value
+        else lookupEnv restEnv varName
     end.
+
+  Fixpoint Feval (env : Env) (expr : FExpr) (max : nat) : @Either (list (string * option FExpr)) Value :=
+    match max with
+    | 0 =>
+        Left (("Error: Maximum recursion depth exceeded", None) :: nil)
+    | S max' =>
+      match expr with
+      | F_Var varName =>
+          match lookupEnv env varName with
+          | Some value => Right value
+          | None =>
+              Left (("Error: Unbound variable", Some (F_Var varName)) :: nil)
+          end
+      | F_Lambda paramName bodyExpr =>
+          Right (V_Closure (F_Lambda paramName bodyExpr) env)
+      | F_Apply funcExpr argExpr =>
+          match Feval env funcExpr max' with
+          | Right (V_Closure (F_Lambda paramName bodyExpr) closureEnv) =>
+              let argValueEither := Feval env (F_Return argExpr) max' in
+              match argValueEither with
+              | Right argValue =>
+                let extendedEnv := ExtendEnv paramName argValue closureEnv in
+                Feval extendedEnv bodyExpr max'
+              | Left err =>
+                  Left 
+                    (("Error: Function argument did not evaluate to a value"
+                     , Some (F_Apply funcExpr argExpr)) :: nil)
+              end
+          | _ =>
+              Left
+                (("Error: Attempted to apply a non-function"
+                 , Some (F_Apply funcExpr argExpr)) :: nil)
+          end
+      | F_Cond condExpr trueExpr falseExpr =>
+          match Beval condExpr env max' with
+          | Some true =>
+              Feval env trueExpr max'
+          | Some false =>
+              Feval env falseExpr max'
+          | _ =>
+              Left
+                (("Error: Condition did not evaluate to a boolean"
+                 , Some (F_Cond condExpr trueExpr falseExpr)) :: nil)
+          end
+      | F_Let varName bindExpr bodyExpr =>
+          let bindValueEither := Feval env bindExpr max' in
+          match bindValueEither with
+          | Right bindValue =>
+            let extendedEnv := ExtendEnv varName bindValue env in
+            Feval extendedEnv bodyExpr max'
+          | Left err =>
+              Left
+                (("Error: Let binding did not evaluate to a value"
+                 , Some (F_Let varName bindExpr bodyExpr)) :: nil)
+          end
+      | F_Return retExpr =>
+          match retExpr with
+          | E_Bool b => 
+              match V_Bool <$> (Beval b env max') with
+              | Some v =>
+                  Right v
+              | None =>
+                  Left
+                    (("Error: Boolean expression did not evaluate to a boolean"
+                     , Some (F_Return retExpr)) :: nil)
+              end
+          | E_Arith a =>
+              match V_Nat <$> (Aeval a env max') with
+              | Some v =>
+                  Right v
+              | None =>
+                  Left
+                    (("Error: Arithmetic expression did not evaluate to a number"
+                     , Some (F_Return retExpr)) :: nil)
+              end
+          end
+      end
+    end
+
+  with Aeval (a : AExpr) (env : Env) (max : nat) : option nat :=
+    match max with
+    | 0 =>
+        None
+    | S max' =>
+      match a with
+      | A_Var n => 
+          match lookupEnv env n with
+          | Some (V_Nat n') =>
+              Some n'
+          | _ =>
+              None
+          end
+      | A_Const n =>
+          Some n
+      | A_Add a1 a2 =>
+          plus <$> (Aeval a1 env max') <*> (Aeval a2 env max')
+      | A_Sub a1 a2 =>
+          minus <$> (Aeval a1 env max') <*> (Aeval a2 env max')
+      | A_Mult a1 a2 =>
+          mult <$> (Aeval a1 env max') <*> (Aeval a2 env max')
+      | A_Func f => 
+          match Feval env f max' with
+          | Right (V_Nat n) =>
+              Some n
+          | _ =>
+              None
+          end
+      end
+    end
+
+  with Beval (b : BExpr) (e : Env) (max : nat) : option bool :=
+    match max with
+    | 0 =>
+        None
+    | S max' =>
+      match b with
+      | B_True =>
+          Some true
+      | B_False =>
+          Some false
+      | B_Not b' =>
+          negb <$> Beval b' e max'
+      | B_And b1 b2 =>
+          andb <$> (Beval b1 e max') <*> (Beval b2 e max')
+      | B_Le b1 b2 =>
+          Nat.leb <$> (Aeval b1 e max') <*> (Aeval b2 e max')
+      end
+    end.
+
+
+  Example bruh := F_Let "factorial" (F_Lambda "n"
+  (F_Cond
+    (B_Le (A_Var "n") (A_Const 1))
+    (F_Return (E_Arith (A_Const 1)))
+    (F_Return (E_Arith (A_Mult
+                (A_Var "n")
+                (A_Func (F_Apply (F_Var "factorial") (E_Arith (A_Sub (A_Var "n") (A_Const 1))))))))))
+  (F_Apply (F_Var "factorial") (E_Arith (A_Const 5))).
+
+  Example bruh2 :=
+    F_Return (E_Arith (A_Func (F_Return (E_Arith (A_Mult (A_Const 2) (A_Const 3)))))).
+
+  Compute Feval EmptyEnv bruh 100.
+  Compute Feval EmptyEnv bruh2 100.
+
+  Definition initialEnv : Env :=
+  ExtendEnv "n" (V_Nat 10)
+    (ExtendEnv "y" (V_Nat 5)
+      EmptyEnv).
+ 
+  Definition initialEnv' : Env :=
+  ExtendEnv "factorial" (V_Closure
+                          (F_Lambda "n"
+                            (F_Cond
+                              (B_Le (A_Var "n") (A_Const 1))
+                              (F_Return (E_Arith (A_Const 1)))
+                              (F_Return
+                                (E_Arith 
+                                (A_Mult
+                                  (A_Var "n")
+                                  (A_Func 
+                                    (F_Apply
+                                      (F_Var "factorial")
+                                        (E_Arith
+                                          (A_Sub
+                                            (A_Var "n")
+                                            (A_Const 1)
+                                          )
+                                        )
+                                      )
+                                    )
+                                  ) 
+                                )
+                              )
+                            )
+                          )
+                        initialEnv)
+                        EmptyEnv.
+
+  Eval simpl in 
+    evalExpr
+    EmptyEnv
+    (F_Cond
+      (B_False)
+      (F_Return (E_Arith (A_Const 1)))
+      (F_Return (E_Arith (A_Const 2))))
+    1000.
+
+  Eval simpl in evalExpr initialEnv' bruh 1000.
+  Eval simpl in Feval bruh initialEnv' 1000.
+
+
+  Eval simpl in evalExpr initialEnv bruh 1000.
 
   Inductive Ceval : CExpr -> State -> State -> Prop :=
     | CE_Skip : forall s,
         Ceval C_Skip s s
-    | CE_Assign : forall s x e n,
-        Aeval e s = Just n ->
-        Ceval (C_Assign x e) s (update_state s x n)
+    | CE_AssignA : forall s x e n,
+        Aeval e s = Some n ->
+        Ceval (C_AssignA x e) s (update_state_A s x (Some n))
+    | CE_AssignL : forall s x e n,
+        Leval e s = Some n ->
+        Ceval (C_AssignL x e) s (update_state_L s x (Some n))
     | CE_Seq : forall c1 c2 s1 s2 s3,
         Ceval c1 s1 s2 ->
         Ceval c2 s2 s3 ->
         Ceval (C_Seq c1 c2) s1 s3
     | CE_IfTrue : forall b c1 c2 s1 s2,
-        Beval b s1 = Just true ->
+        Beval b s1 = Some true ->
         Ceval c1 s1 s2 ->
         Ceval (C_If b c1 c2) s1 s2
     | CE_IfFalse : forall b c1 c2 s1 s2,
-        Beval b s1 = Just false ->
+        Beval b s1 = Some false ->
         Ceval c2 s1 s2 ->
         Ceval (C_If b c1 c2) s1 s2
     | CE_WhileFalse : forall b c s,
-        Beval b s = Just false ->
+        Beval b s = Some false ->
         Ceval (C_While b c) s s
     | CE_WhileTrue : forall b c s1 s2 s3,
-        Beval b s1 = Just true ->
+        Beval b s1 = Some true ->
         Ceval c s1 s2 ->
         Ceval (C_While b c) s2 s3 ->
         Ceval (C_While b c) s1 s3.
+
+
+  Fixpoint list_update_at_index (l : list nat) (n : nat) (v : nat) : list nat :=
+    match l with
+    | nil => nil
+    | cons x xs => match n with
+                   | O => cons v xs
+                   | S n' => cons x (list_update_at_index xs n' v)
+                   end
+    end.
 
   Fixpoint Ceval_step (e : CExpr) (s : State) (max : nat) : State :=
     match max with
@@ -154,35 +340,78 @@ Module Semantics.
     | S max' =>
       match e with
       | C_Skip => s
-      | C_Assign c a =>
-          match Aeval a s with
-          | Just n => update_state s c n
-          | Nothing => s
+      | C_AssignA x e =>
+          match Aeval e s with
+          | Some n => update_state_A s x (Some n)
+          | None => s
           end
-      | C_Seq c1 c2 => Ceval_step c2 (Ceval_step c1 s (max' - 1)) (max' - 1)
+      | C_AssignL x e =>
+          match Leval e s with
+          | Some n => update_state_L s x (Some n)
+          | None => s
+          end
+      | C_Seq c1 c2 => Ceval_step c2 (Ceval_step c1 s max') max'
       | C_If b c1 c2 =>
           match Beval b s with
-          | Just b' => if b' then Ceval_step c1 s (max' - 1) else Ceval_step c2 s (max' - 1)
+          | Some b' => if b' then Ceval_step c1 s max' else Ceval_step c2 s max'
           | Nohting => s
           end
       | C_While b c =>
           match Beval b s with
-          | Just b' => if b' then Ceval_step (C_Seq c (C_While b c)) s (max' - 1) else s
-          | Nothing => s
+          | Some b' => if b' then Ceval_step (C_Seq c (C_While b c)) s max' else s
+          | None => s
+          end
+      | C_Foreach x l c =>
+          match Leval l s with
+          | Some l' => 
+              fold_left (fun s' a => Ceval_step (C_Seq (C_AssignA x (A_Const a)) c) s' max') l' s
+          | None => s
+          end
+      | C_Print a => 
+          match Aeval a s with
+          | Some n => update_state_P s n
+          | None => s
+          end
+      | C_ListUpdate n i v =>
+          match Aeval i s, Aeval v s with
+          | Some i', Some v' => 
+              match L_State s n with
+              | Some l => update_state_L s n (Some (list_update_at_index l i' v'))
+              | None => s
+              end
+          | _, _ => s
           end
       end
     end.
 
   Open Scope string_scope.
   Open Scope com_scope.
-  Open Scope nat_scope.
 
-  Example ex1 : CExpr :=
-    <{
-      while "x" < 5 do
-        "x" := "x" + 1
-      end
-    }>.
+  Definition swap :=
+    Ceval_step <{
+      "xs" @:= [1, 2, 3, 4, 5];
+      "ys" @:= [6, 7, 8, 9, 10];
+      "i" := 0;
+      "j" := 0;
+      foreach "x" in "xs" do
+        foreach "y" in "ys" do
+          if "x" < "y" then
+            "tmp" := "x";
+            (update "xs"["i"] to "y");
+            (update "ys"[A_Id "j"] to "tmp")
+          else
+            skip
+          end;
+          "j" := "j" + 1
+        done;
+        "i" := "i" + 1
+      done
+    }> empty_state 10000.
+
+  Compute A_State swap "i".
+  Compute A_State swap "j".
+  Compute L_State swap "xs".
+  Compute L_State swap "ys".
 
 End Semantics.
 
@@ -191,10 +420,10 @@ Import Semantics.
 
 Extraction Language Haskell.
 
-Extract Inductive Maybe => "Prelude.Maybe" ["Prelude.Nothing" "Prelude.Just"].
+Extract Inductive option => "Prelude.Maybe" ["Prelude.Just" "Prelude.Nothing"].
 Extract Inductive nat => "Prelude.Integer" ["0" "Prelude.succ"]
   "(\fO fS n -> if n Prelude.== 0 then fO () else fS (n Prelude.- 1))".
-Extract Inlined Constant fmap => "(Prelude.<$>)".
+Extract Inlined Constant option_map => "(Prelude.<$>)".
 Extract Inlined Constant ap => "(Prelude.<*>)".
 
-Extraction "asd.hs" test_prog_eval.
+Extraction "Haskell.hs" Ceval_step swap.
